streamAE interface

src/tls/StreamAE.fsti
@@ -11,12 +11,14 @@ open FStar.Bytes
 open FStar.UInt32
 open Mem
 open Pkg
-  
+
+
 type llbytes (lmax:nat) = b:bytes{length b <= lmax}
 
 val plain: i:I.id -> lmax:AEAD.plainLen -> Type0
 
 type cipher (i:I.id) (lmax:AEAD.plainLen) = llbytes lmax
+
 
 val stream_entry : i:I.id -> Type0
 
@@ -28,13 +30,45 @@ val mk_entry (#i:I.id) :
     stream_entry i
 
 
-val stream_state: I.id -> I.rw -> Type0
+//val stream_state: I.id -> I.rw -> Type0
 
+val stream_writer: I.id -> Type0
+val stream_reader: #i:I.id -> w:stream_writer i -> Type0
+
+val wctrT: #i:I.id -> w:stream_writer i -> mem -> GTot nat
+val wctr: #i:I.id -> w:stream_writer i -> ST UInt32.t
+  (requires fun h0 -> True)
+  (ensures fun h0 c h1 -> h0 == h1 /\ UInt32.v c = wctrT w h1)
+  
+val rctrT: #i:I.id -> #w:stream_writer i -> stream_reader w -> h:mem ->
+  GTot (n:nat{n <= wctrT w h})
+val rctr: #i:I.id -> #w:stream_writer i -> r:stream_reader w -> ST UInt32.t
+  (requires fun h0 -> True)
+  (ensures fun h0 c h1 -> h0 == h1 /\ UInt32.v c = rctrT r h1)
+
+val wlog: #i:I.id -> w:stream_writer i -> h:mem -> GTot (s:Seq.seq (stream_entry i){wctrT w h == Seq.length s})
+
+let prefix (#i:I.id) (w:stream_writer i) (h:mem) (k:nat{k <= wctrT w h}) =
+  Seq.Base.slice (wlog w h) 0 k
+
+val rlog: #i:I.id -> #w:stream_writer i -> r:stream_reader w -> h:mem ->
+  GTot (s:Seq.seq (stream_entry i){s == prefix w h (rctrT r h)})
+
+(*
 val ctrT: #i:I.id -> #rw:I.rw -> wr:stream_state i rw -> mem -> GTot UInt32.t
 
-val log: #i:I.id -> #rw:I.rw -> wr:stream_state i rw -> mem -> GTot (Seq.seq (stream_entry i))
+val log: #i:I.id -> #rw:I.rw -> wr:stream_state i rw -> h:mem -> GTot (s:Seq.seq (stream_entry i){UInt32.v (ctrT wr h) == Seq.length s})
+
+let log_inv (#i:I.id) (rw:stream_state i) (h:mem) =
+    log (rw Reader) h == prefix (log (rw Writer) h) (ctrT (rw Reader) h) 
 
 val invariant: #i:I.id -> #rw:I.rw -> stream_state i rw -> mem -> Type0
+*)
+
+val invariant: #i:I.id -> w:stream_writer i -> mem -> Type0
+
+let rinvariant (#i:I.id) (#w:stream_writer i) (r:stream_reader w) (h:mem) =
+  invariant w h
 
 type info' = {
   alg: I.aeadAlg;
@@ -45,80 +79,99 @@ type info' = {
 type info (i:I.id) =
   info:info'{I.aeadAlg_of_id i == info.alg}
 
-val shared_footprint: rset
+val footprint: #i:I.id -> stream_writer i -> s:rset
 
-val footprint: #i:I.id -> #rw:I.rw -> stream_state i rw -> s:rset{Set.disjoint s shared_footprint}
+val shared_footprint: #i:I.id -> w:stream_writer i -> s:rset{Set.disjoint s (footprint w)}
 
-val log_region: #i:I.id -> #rw:I.rw -> stream_state i rw -> subrgn tls_tables_region
+let rfootprint (#i:I.id) (#w:stream_writer i) (r:stream_reader w): GTot rset =
+  shared_footprint w
 
+//val log_region: #i:I.id -> #rw:I.rw -> stream_state i rw -> subrgn tls_tables_region
+ 
 
-
-val frame_invariant: #i:I.id -> #rw:I.rw -> s:stream_state i rw -> h0:mem -> r:rid -> h1:mem ->
+val frame_invariant: #i:I.id -> w:stream_writer i -> h0:mem -> ri:rid -> h1:mem ->
   Lemma
   (requires
-    (invariant s h0 /\
-    modifies_one r h0 h1 /\
-    ~(Set.mem r (footprint s)) /\
-    ~(Set.mem r (shared_footprint))))
-  (ensures invariant s h1)
+    (invariant w h0 /\
+    modifies_one ri h0 h1 /\
+    ~(Set.mem ri (footprint w)) /\
+    ~(Set.mem ri (shared_footprint w))))
+  (ensures invariant w h1)
 
-val frame_log: #i:I.id -> #rw:I.rw -> s:stream_state i rw -> l:Seq.seq (stream_entry i) ->
-  h0:mem -> r:rid -> h1:mem ->
+val rframe_invariant: #i:I.id -> #w:stream_writer i -> r:stream_reader w -> h0:mem -> ri:rid -> h1:mem ->
+  Lemma
+  (requires
+    (rinvariant r h0 /\
+    modifies_one ri h0 h1 /\
+    ~(Set.mem ri (rfootprint r))))
+  (ensures rinvariant r h1)
+
+val frame_log: #i:I.id -> w:stream_writer i -> l:Seq.seq (stream_entry i) ->
+  h0:mem -> ri:rid -> h1:mem ->
   Lemma
   (requires
     Flag.safeId i /\
-    log s h0 == l /\
-    modifies_one r h0 h1 /\
-    ~(Set.mem r (footprint s)))
-  (ensures log s h1 == l)
+    wlog w h0 == l /\
+    modifies_one ri h0 h1 /\
+    ~(Set.mem ri (footprint w)))
+  (ensures wlog w h1 == l)
 
 
 val create: i:I.id -> u:info i ->
-  ST (stream_state i I.Writer)
-  (requires fun h0 -> disjoint u.shared u.local)
-  (ensures fun h0 s h1 ->
-    invariant s h1 /\
-    shared_footprint == Set.singleton u.shared /\
-    footprint s == Set.singleton u.local /\
-    log_region s == u.local /\
+  ST (stream_writer i)
+  (requires fun h0 -> 
+    disjoint u.shared u.local)
+  (ensures fun h0 w h1 ->
+    invariant w h1 /\
+    footprint w == Set.singleton u.local /\
+    shared_footprint w == Set.singleton u.shared /\
     modifies_none h0 h1 /\
     Flag.safeId i ==>
-      (log s h1 == Seq.empty /\
-      ctrT s h1 == 0ul)
+      (wlog w h1 == Seq.empty /\
+      wctrT w h1 == 0)
   )
 
-let reader_footprint (#i:I.id) (w:stream_state i I.Writer) : GTot rset =
-  shared_footprint
-  
-val createReader: #i:I.id -> w:stream_state i I.Writer ->
-  ST (stream_state i I.Reader)
+val coerce: parent:rgn -> i:I.id -> u:info i ->
+  ST (stream_writer i)
+  (requires fun h0 -> 
+    ~ (Flag.safeId i) /\ disjoint u.shared u.local)
+  (ensures fun h0 w h1 ->
+    invariant w h1 /\
+    footprint w == Set.singleton u.local /\
+    shared_footprint w == Set.singleton u.shared /\
+    modifies_none h0 h1)
+
+
+val createReader: #i:I.id -> w:stream_writer i ->
+  ST (stream_reader w)
   (requires fun h0 -> invariant w h0)
   (ensures fun h0 r h1 ->
-    invariant r h1 /\
+    rinvariant r h1 /\
     modifies_none h0 h1 /\
-    log_region r == log_region w /\
-    footprint r == reader_footprint w /\
     Flag.safeId i ==>
-      (log r h1 == Seq.empty /\
-      ctrT r h1 == 0ul)
+      (rlog r h1 == Seq.empty /\
+      rctrT r h1 == 0)
   )
 
-val incrementable : #i:I.id -> #rw:I.rw -> stream_state i rw -> mem -> Type0
+val incrementable: #i:I.id -> stream_writer i  -> mem -> Type0
+
+//val rincrementable: #i:I.id -> #w:stream_writer i -> r:stream_reader w -> h:mem -> Type0
+
 
 val encrypt
   (#i:I.id)
-  (s:stream_state i I.Writer)
+  (w:stream_writer i)
   (ad:AEAD.adata)
   (lmax:AEAD.plainLen)
   (p:plain i lmax):
   ST (cipher i lmax)
-  (requires fun h0 -> incrementable s h0 /\ invariant s h0)
+  (requires fun h0 -> incrementable w h0 /\ invariant w h0)
   (ensures fun h0 c h1 ->
-    U32.v (ctrT s h1) == U32.v (ctrT s h0) + 1 /\ 
+    wctrT w h1 == wctrT w h0 + 1 /\ 
     (Flag.safeId i ==> (
-      log s h1 == Seq.cons (mk_entry ad p c) (log s h0))) /\
-    invariant s h1 /\
-    modifies (Set.union (footprint s) shared_footprint) h0 h1)
+      wlog w h1 == Seq.snoc (wlog w h0) (mk_entry ad p c))) /\
+    invariant w h1 /\
+    modifies (Set.union (footprint w) (shared_footprint w)) h0 h1)
 
 val adata_of_entry: #i:I.id -> stream_entry i -> GTot AEAD.adata
 
@@ -131,22 +184,23 @@ let matches (#i:I.id) (e:stream_entry i) (ad:AEAD.adata) (lmax:AEAD.plainLen) (c
 
 val decrypt
   (#i:I.id)
-  (s:stream_state i I.Reader)
+  (#w:stream_writer i)
+  (r:stream_reader w)
   (ad:AEAD.adata)
   (lmax:AEAD.plainLen)
   (c:cipher i lmax):
   ST (option (plain i lmax))
-  (requires fun h0 -> incrementable s h0 /\ invariant s h0)
+  (requires fun h0 -> rinvariant r h0)
   (ensures fun h0 res h1 ->
-    invariant s h1 /\
-    modifies (footprint s) h0 h1 /\
+    rinvariant r h1 /\
+    modifies (rfootprint r) h0 h1 /\
     (Flag.safeId i ==> (
-      let j = U32.v (ctrT s h0) in
-      let lg = log s h0 in
-      if j < Seq.length lg && matches (Seq.index lg j) ad lmax c then
+      let j = rctrT r h0 in
+      let lg = wlog w h0 in
+      if j < wctrT w h0 && matches (Seq.index lg j) ad lmax c then
         (Some? res /\
         Seq.index lg j == mk_entry ad (Some?.v res) c /\
-        U32.v (ctrT s h1) == j + 1)
+        rctrT r h1 == j + 1)
       else
         res == None)))
         
